Proving translation properties. Needs to relax typing

coq/coq/Translation.v
@@ -8,12 +8,89 @@ Require Import Sorting.Sorted.
 Require Export Infrastructure.
 
 
+(* Source types to type indexes *)
+Notation "|| A ||" := (type2index A) (at level 50, A at next level). (* 1 is too high *)
+
+
+(* Concatenate two record types without any checking *)
+
+Fixpoint ttyp_concat_simpl (A: ttyp) (B: ttyp) :=
+  match A with
+  | ttyp_top => B
+  | ttyp_rcd l At Bt => ttyp_rcd l At (ttyp_concat_simpl Bt B)
+  | _ => ttyp_top
+  end.
+
+Lemma lookup_concat_simpl : forall i A B T,
+    Tlookup i A = Some T ->
+    Tlookup i (ttyp_concat_simpl A B) = Tlookup i A.
+Proof.
+  introv LK. gen i T B.
+  induction A; intros; simpl in LK; inverts LK.
+  case_if*.
+  - inverts* H0.
+    subst. simpl. case_if*.
+  - simpl. case_if*.
+Qed.
+
+
+Lemma lookup_concat_simpl_none : forall i A B,
+    Tlookup i A = None -> rec_typ A ->
+    Tlookup i (ttyp_concat_simpl A B) = Tlookup i B.
+Proof.
+  introv LK HR. gen i B.
+  induction A; intros; simpl; try solve_by_invert; eauto.
+  - inverts* HR. inverts LK. case_if.
+    forwards* Heq: IHA2.
+Qed.
+
+Lemma rcd_typ_concat_simpl : forall T1 T2,
+    rec_typ T1 -> rec_typ T2 ->
+    rec_typ (ttyp_concat_simpl T1 T2).
+Proof with eauto.
+  introv WF1 WF2.
+  induction WF1...
+  - simpl...
+Qed.
+
+(* Source types to target types *)
+
+Reserved Notation "[[ A ]]" (at level 5, A at next level).
+
+Fixpoint styp2ttyp_raw (A: typ) : ttyp :=
+  match A with
+  | typ_top => ttyp_top
+  | typ_bot => ttyp_bot
+  | typ_base =>  ttyp_base
+  | typ_arrow B1 B2 => ttyp_arrow ([[ B1 ]]) ([[ B2 ]])
+  | _ => ttyp_top (* for rcd and intersections *)
+  end
+where "[[ A ]]" := (styp2ttyp_raw A).
+
 Reserved Notation "|[ A ]|" (at level 5, A at next level).
 
-Fixpoint styp2ttyp (A: typ) : ttyp := ttyp_base
+Fixpoint styp2ttyp (A: typ) : ttyp :=
+  match A with
+  | typ_top => ttyp_top
+  | typ_bot => ttyp_rcd (|| A ||) [[ A ]] ttyp_top
+  | typ_base => ttyp_rcd (|| A ||) [[ A ]] ttyp_top
+  | typ_arrow B1 B2 => ttyp_rcd (|| A ||) [[ A ]] ttyp_top
+  | typ_rcd l A' => ttyp_rcd (|| A ||) (|[ A' ]|) ttyp_top
+  | typ_and A1 A2 => ttyp_concat_simpl (|[ A1 ]|) (|[ A2 ]|)
+  end
 where "|[ A ]|" := (styp2ttyp A).
 
-Notation "|| A ||" := (type2index A) (at level 1, A at next level). (* too high *)
+(* Fixpoint styp2ttyp (A: typ) : ttyp := *)
+(*   match A with *)
+(*   | typ_top => ttyp_top *)
+(*   | typ_bot => ttyp_rcd (|| A ||) ttyp_bot ttyp_top *)
+(*   | typ_base => ttyp_rcd (|| A ||) ttyp_base ttyp_top *)
+(*   | typ_arrow B1 B2 => ttyp_rcd (|| A ||) (ttyp_arrow (|[ B1 ]|) (|[ B2 ]|)) ttyp_top *)
+(*   | typ_rcd l A' => ttyp_rcd (|| A ||) (|[ A' ]|) ttyp_top *)
+(*   | typ_and A1 A2 => ttyp_concat_simpl (|[ A1 ]|) (|[ A2 ]|) *)
+(*   end *)
+(* where "|[ A ]|" := (styp2ttyp A). *)
+
 
 (* Properties of translation (to type index) functions *)
 (* Lemma tindex_trans_arrow : forall A B, *)
@@ -25,8 +102,40 @@ Notation "|| A ||" := (type2index A) (at level 1, A at next level). (* too high 
 
 (* Properties of translation (to target type) functions *)
 
+#[local] Hint Constructors wf_typ : core.
+
+
+Lemma translate_to_record_types : forall A,
+    rec_typ |[ A ]|.
+Proof with eauto using rcd_typ_concat_simpl.
+  introv. induction A; simpl...
+Qed.
+
+Lemma lookup_concat_simpl_none : forall i A B,
+    Tlookup l |[A]| = Some  -> rec_typ A ->
+    Tlookup i (ttyp_concat_simpl A B) = Tlookup i B.
+Proof.
+  introv LK HR. gen i B.
+  induction A; intros; simpl; try solve_by_invert; eauto.
+  - inverts* HR. inverts LK. case_if.
+    forwards* Heq: IHA2.
+Qed.
+
+
 Lemma ttyp_trans_wf : forall A,
     wf_typ |[A]|.
+Proof with intuition eauto using rcd_typ_concat_simpl.
+  introv. induction A; simpl...
+  - lets HR1: translate_to_record_types A1.
+    lets HR2: translate_to_record_types A2.
+    induction* HR1.
+    + inverts* IHA1.
+      simpl...
+      * forwards* Heq: lookup_concat_simpl H.
+        rewrite H in Heq...
+      * forwards* Heq: lookup_concat_simpl_none |[ A2 ]| H...
+        rewrite H in Heq...
+        applys* WF_Rcd...
 Admitted.
 
 (* Typ-TopAbs requires no ord *)
@@ -35,21 +144,21 @@ Lemma ttyp_trans_ord_top : forall A,
 Admitted.
 
 Lemma ttyp_trans_ord_ntop : forall A,
-    ord A -> ~ toplike A -> exists B, |[A]| = ttyp_rcd ||A|| B ttyp_top /\ wf_typ B.
+    ord A -> ~ toplike A -> exists B, |[A]| = (ttyp_rcd (||A||) B ttyp_top) /\ wf_typ B.
 Admitted.
 
 Lemma ttyp_trans_base :
-    |[typ_base]| = ttyp_rcd ||typ_base|| ttyp_base ttyp_top.
+    |[typ_base]| = ttyp_rcd (||typ_base||) ttyp_base ttyp_top.
 Admitted.
 
 Lemma ttyp_trans_ord_ntop_arrow : forall A A',
     (* ord A -> ~ toplike A -> *) (* S-arrow requires no precondition *)
-    |[(typ_arrow A' A)]| = ttyp_rcd (ti_arrow || A ||) (ttyp_arrow |[A']| |[A]|) ttyp_top.
+    |[(typ_arrow A' A)]| = ttyp_rcd (||typ_arrow A' A||) (ttyp_arrow |[A']| |[A]|) ttyp_top.
 Admitted.
 
 Lemma ttyp_trans_rcd : forall l A,
     (* ord A -> ~ toplike A -> *) (* S-arrow requires no precondition *)
-    |[(typ_rcd l A)]| = ttyp_rcd (ti_rcd l || A ||) |[A]| ttyp_top.
+    |[(typ_rcd l A)]| = ttyp_rcd (||(typ_rcd l A)||) |[A]| ttyp_top.
 Admitted.
 
 Lemma ttyp_trans_and : forall A B C,
@@ -59,8 +168,4 @@ Admitted.
 (* Properties about type translation *)
 Lemma concat_source_intersection : forall A B,
     concat_typ |[ A ]| |[ B ]| |[ (typ_and A B) ]|.
-Admitted.
-
-Lemma translate_to_record_types : forall A,
-    rec_typ |[ A ]|.
 Admitted.
